Examples/Scroll/Keccak/Gates/All.lean
@@ -2,6 +2,8 @@ import Examples.Scroll.Keccak.Gates.AbsorbResult
 import Examples.Scroll.Keccak.Gates.AbsorbResultCopy.All
 import Examples.Scroll.Keccak.Gates.AbsorbStateCopy.All
 import Examples.Scroll.Keccak.Gates.AbsorbVerifyInput.All
+import Examples.Scroll.Keccak.Gates.HashRlcCheck
 import Examples.Scroll.Keccak.Gates.NextRowCheck.All
 import Examples.Scroll.Keccak.Gates.Split
 import Examples.Scroll.Keccak.Gates.SplitUniform.All
+import Examples.Scroll.Keccak.Gates.SqueezeVerifyPacked.All
