Examples/Scroll/Keccak/Gates/HashRlcCheck.lean
@@ -1,0 +1,55 @@
+import Examples.Scroll.Keccak.CellManager
+import Examples.Scroll.Keccak.Spec.ComposeRlc
+import Examples.Scroll.Keccak.Spec.HashRlc
+import Examples.Scroll.Keccak.Spec.Program
+
+-- def expr (l: List (ZMod P)) (r k: ZMod P) (hk: k = r ^ (l.length)) :=
+--   (l.enum.map (λ (idx, val) => val * (r ^ idx))).sum
+-- lemma base (val val' r: ZMod P): val + val' * r = expr [val, val'] r (r*r) (by simp [List.length, pow_two]) := by
+--   simp [expr, List.map]
+-- lemma cons: expr l r (k*r) hk + val * (k * r) = expr (l ++ [val]) r (k*r*r) (by simp [hk, pow_add]) := by
+--   simp [expr]
+--   rewrite [List.enum_append, List.map_append, List.sum_append]
+--   congr
+--   simp [hk]
+
+-- lemma to_rlc: expr l r k hk = Keccak.ComposeRlc.expr l r := by
+--   unfold Keccak.ComposeRlc.expr expr
+--   simp [List.sum_eq_foldr, ←List.foldl_eq_foldr]
+
+
+
+namespace Keccak
+  namespace Gates
+    namespace HashRlcCheck
+
+      lemma gate_124_hash_rlc_check (c: ValidCircuit P P_Prime) (h_fixed: c.1.Fixed = fixed_func c) (hgate: gate_124 c) (h_n: 263 < c.n) :
+        start_new_hash c 300 → ComposeRlc.expr (hash_bytes_le c 25) (c.get_challenge 0 0) = hash_rlc c 300
+      := by
+        unfold gate_124 at hgate
+        intro h_start
+        simp [start_new_hash, ValidCircuit.get_fixed, h_fixed, fixed_func, fixed_func_col_1, zmod_not_zero_eq_one, P_Prime, is_final] at h_start
+        replace hgate := hgate 300
+        simp [ValidCircuit.get_fixed, h_fixed, Selectors.q_round_last_one, one_mul, h_start] at hgate
+        simp [fixed_func, fixed_func_col_1] at hgate
+        replace hgate := eq_neg_of_add_eq_zero_left hgate
+        rewrite [neg_involutive] at hgate
+        rewrite [to_hash_rlc] at hgate
+        rewrite [←hgate]
+        clear hgate
+        simp only [hash_bytes_le, hash_bytes, cell_manager, List.reverse, List.reverseAux]
+        norm_num
+        simp only [ValidCircuit.get_advice_wrapped, Nat.reduceAdd]
+        have h (k: ℕ): k < 49 → k % c.n = k := by
+          intro hk
+          rw [Nat.mod_eq_of_lt]
+          linarith
+        simp [h]
+        simp [Nat.sub_add_comm]
+        unfold ComposeRlc.expr
+        rewrite [List.foldl_cons]
+        simp
+
+    end HashRlcCheck
+  end Gates
+end Keccak
