Examples/Scroll/Keccak/Spec/ComposeRlc.lean
@@ -1,0 +1,8 @@
+import Examples.Scroll.Keccak.Spec.Program
+
+namespace Keccak
+  namespace ComposeRlc
+    lemma to_rlc_base (val r: ZMod P): val * k + val' * (k * r) = expr [val*k, val'*k] r := by simp [expr, mul_assoc]
+    lemma to_rlc_cons: expr [val] r + val' * r = expr [val, val'] r := by simp [expr]
+  end ComposeRlc
+end Keccak
