Examples/Scroll/Keccak/Spec/HashRlc.lean
@@ -1,0 +1,5 @@
+import Examples.Scroll.Keccak.Spec.Program
+
+namespace Keccak
+  lemma to_hash_rlc: c.get_advice 3 row = hash_rlc c row := rfl
+end Keccak
